{
 "cells": [
  {
   "cell_type": "markdown",
   "id": "692a5bd0",
   "metadata": {},
   "source": [
    "# Primitive Recursive Functions\n",
    "https://claude.ai/chat/135a6c49-0e7d-4cd3-83d3-23369a95d777\n",
    "\n"
   ]
  },
  {
   "cell_type": "code",
   "execution_count": 3,
   "id": "300f8be5",
   "metadata": {},
   "outputs": [
    {
     "name": "stdout",
     "output_type": "stream",
     "text": [
      "=== Basic Projection Examples ===\n",
      "P_1^3(7, 42, 15) = 7\n",
      "P_2^3(7, 42, 15) = 42\n",
      "P_3^3(7, 42, 15) = 15\n",
      "P_1^2(100, 200) = 100\n",
      "P_2^2(100, 200) = 200\n",
      "\n",
      "=== Function Composition Example ===\n",
      "f(5, 99) = S(P_1^2(5, 99)) = S(5) = 6\n",
      "g(10, 7, 30) = S(P_2^3(10, 7, 30)) = S(7) = 8\n",
      "h(6, 100) = P_1^2(6, 100) + P_1^2(6, 100) = 6 + 6 = 12\n",
      "\n",
      "=== Identity Functions using Projections ===\n",
      "P_1^1(42) = 42 (identity function)\n",
      "\n",
      "=== Practical Analogy ===\n",
      "data = (10, 20, 30)\n",
      "data[0] is like P_1^3: 10\n",
      "data[1] is like P_2^3: 20\n",
      "data[2] is like P_3^3: 30\n"
     ]
    }
   ],
   "source": [
    "# Projection functions - extract specific arguments from a tuple\n",
    "\n",
    "def projection(i, n):\n",
    "    \"\"\"\n",
    "    Returns a projection function P_i^n that takes n arguments \n",
    "    and returns the i-th argument (1-indexed)\n",
    "    \"\"\"\n",
    "    def proj_func(*args):\n",
    "        if len(args) != n:\n",
    "            raise ValueError(f\"Expected {n} arguments, got {len(args)}\")\n",
    "        if i < 1 or i > n:\n",
    "            raise ValueError(f\"Index {i} out of range for {n} arguments\")\n",
    "        return args[i - 1]  # Convert to 0-indexed for Python\n",
    "    \n",
    "    return proj_func\n",
    "\n",
    "# Create some specific projection functions\n",
    "P_1_3 = projection(1, 3)  # First of three arguments\n",
    "P_2_3 = projection(2, 3)  # Second of three arguments  \n",
    "P_3_3 = projection(3, 3)  # Third of three arguments\n",
    "\n",
    "P_1_2 = projection(1, 2)  # First of two arguments\n",
    "P_2_2 = projection(2, 2)  # Second of two arguments\n",
    "\n",
    "# Examples of using projection functions\n",
    "print(\"=== Basic Projection Examples ===\")\n",
    "print(f\"P_1^3(7, 42, 15) = {P_1_3(7, 42, 15)}\")  # Should be 7\n",
    "print(f\"P_2^3(7, 42, 15) = {P_2_3(7, 42, 15)}\")  # Should be 42\n",
    "print(f\"P_3^3(7, 42, 15) = {P_3_3(7, 42, 15)}\")  # Should be 15\n",
    "\n",
    "print(f\"P_1^2(100, 200) = {P_1_2(100, 200)}\")    # Should be 100\n",
    "print(f\"P_2^2(100, 200) = {P_2_2(100, 200)}\")    # Should be 200\n",
    "\n",
    "# Example: Why projections are useful in function composition\n",
    "print(\"\\n=== Function Composition Example ===\")\n",
    "\n",
    "def successor(n):\n",
    "    \"\"\"Successor function: S(n) = n + 1\"\"\"\n",
    "    return n + 1\n",
    "\n",
    "def zero():\n",
    "    \"\"\"Zero function: returns 0\"\"\"\n",
    "    return 0\n",
    "\n",
    "# Suppose we want to define a function f(x, y) = S(x) \n",
    "# (successor of first argument, ignoring second)\n",
    "# We compose successor with the first projection:\n",
    "\n",
    "def f(x, y):\n",
    "    \"\"\"f(x, y) = S(P_1^2(x, y)) = S(x) = x + 1\"\"\"\n",
    "    return successor(P_1_2(x, y))\n",
    "\n",
    "print(f\"f(5, 99) = S(P_1^2(5, 99)) = S(5) = {f(5, 99)}\")\n",
    "\n",
    "# Another example: g(x, y, z) = S(P_2^3(x, y, z)) = y + 1\n",
    "def g(x, y, z):\n",
    "    \"\"\"g(x, y, z) = S(P_2^3(x, y, z)) = y + 1\"\"\"\n",
    "    return successor(P_2_3(x, y, z))\n",
    "\n",
    "print(f\"g(10, 7, 30) = S(P_2^3(10, 7, 30)) = S(7) = {g(10, 7, 30)}\")\n",
    "\n",
    "# Example: Using same argument twice\n",
    "# h(x, y) = x + x (add first argument to itself)\n",
    "def add(a, b):\n",
    "    \"\"\"Simple addition\"\"\"\n",
    "    return a + b\n",
    "\n",
    "def h(x, y):\n",
    "    \"\"\"h(x, y) = P_1^2(x, y) + P_1^2(x, y) = x + x\"\"\"\n",
    "    return add(P_1_2(x, y), P_1_2(x, y))\n",
    "\n",
    "print(f\"h(6, 100) = P_1^2(6, 100) + P_1^2(6, 100) = 6 + 6 = {h(6, 100)}\")\n",
    "\n",
    "print(\"\\n=== Identity Functions using Projections ===\")\n",
    "# Special case: projection functions with n=1 are identity functions\n",
    "P_1_1 = projection(1, 1)\n",
    "print(f\"P_1^1(42) = {P_1_1(42)} (identity function)\")\n",
    "\n",
    "print(\"\\n=== Practical Analogy ===\")\n",
    "# Think of projections like array/tuple indexing\n",
    "data = (10, 20, 30)\n",
    "print(f\"data = {data}\")\n",
    "print(f\"data[0] is like P_1^3: {data[0]}\")\n",
    "print(f\"data[1] is like P_2^3: {data[1]}\")  \n",
    "print(f\"data[2] is like P_3^3: {data[2]}\")\n"
   ]
  },
  {
   "cell_type": "markdown",
   "id": "3ae6332c",
   "metadata": {},
   "source": [
    "# Addition with Primitive Recursive Functions"
   ]
  },
  {
   "cell_type": "code",
   "execution_count": 4,
   "id": "19813597",
   "metadata": {},
   "outputs": [
    {
     "name": "stdout",
     "output_type": "stream",
     "text": [
      "=== Step 1: Understanding the recursive definition ===\n",
      "We want to define sum(a, b) using primitive recursion:\n",
      "sum(a, 0) = a\n",
      "sum(a, n+1) = S(sum(a, n))\n",
      "\n",
      "=== Step 2: Formal primitive recursive definition ===\n",
      "In primitive recursion, we define a function f by:\n",
      "f(0, x₁, ..., xₖ) = g(x₁, ..., xₖ)         [base case]\n",
      "f(n+1, x₁, ..., xₖ) = h(n, f(n,x₁,...,xₖ), x₁, ..., xₖ)  [recursive case]\n",
      "\n",
      "For sum(a, b), we have:\n",
      "- f is our sum function\n",
      "- We're recursing on the second argument b\n",
      "- x₁ = a (the first argument)\n",
      "- So: sum(a, 0) = g(a) and sum(a, n+1) = h(n, sum(a,n), a)\n",
      "\n",
      "=== Step 3: Base case function g ===\n",
      "g(a) = P_1^1(a) = a\n",
      "This handles: sum(a, 0) = a\n",
      "Example: g(5) = 5\n",
      "\n",
      "=== Step 4: Recursive case function h ===\n",
      "h(n, recursive_result, a) = S(P_2^3(n, recursive_result, a))\n",
      "This handles: sum(a, n+1) = S(sum(a, n))\n",
      "The P_2^3 extracts the recursive_result (sum(a, n))\n",
      "Then S() gives us the successor\n",
      "\n",
      "=== Step 5: Testing our primitive recursive sum ===\n",
      "prim_recursive_sum(3, 0) = 3 (expected 3) ✓\n",
      "prim_recursive_sum(3, 1) = 4 (expected 4) ✓\n",
      "prim_recursive_sum(3, 2) = 5 (expected 5) ✓\n",
      "prim_recursive_sum(5, 4) = 9 (expected 9) ✓\n",
      "prim_recursive_sum(0, 7) = 7 (expected 7) ✓\n",
      "prim_recursive_sum(7, 0) = 7 (expected 7) ✓\n",
      "\n",
      "=== Step 6: Trace through sum(3, 2) ===\n",
      "sum(3, 2):\n",
      "  Since 2 ≠ 0, we use recursive case with n=1\n",
      "  = h(1, sum(3, 1), 3)\n",
      "  \n",
      "  First we need sum(3, 1):\n",
      "    Since 1 ≠ 0, we use recursive case with n=0\n",
      "    = h(0, sum(3, 0), 3)\n",
      "    \n",
      "    First we need sum(3, 0):\n",
      "      Since 0 = 0, we use base case\n",
      "      = g(3) = P_1^1(3) = 3\n",
      "    \n",
      "    So h(0, 3, 3) = S(P_2^3(0, 3, 3)) = S(3) = 4\n",
      "    Therefore sum(3, 1) = 4\n",
      "  \n",
      "  Now h(1, 4, 3) = S(P_2^3(1, 4, 3)) = S(4) = 5\n",
      "  Therefore sum(3, 2) = 5\n",
      "\n",
      "=== Step 7: The key insight ===\n",
      "Addition is primitive recursive because it can be built using only:\n",
      "1. Basic functions: zero(), successor(), projections\n",
      "2. Composition: plugging functions into other functions\n",
      "3. Primitive recursion: the specific pattern above\n",
      "\n",
      "No 'loops' or 'general recursion' needed - just this constrained form!\n",
      "\n",
      "=== Verification: Only primitive operations used ===\n",
      "✓ g(a) = P_1^1(a) - uses projection\n",
      "✓ h(n,r,a) = S(P_2^3(n,r,a)) - uses successor and projection\n",
      "✓ Primitive recursion pattern followed exactly\n",
      "✓ No general recursion, loops, or unbounded search\n"
     ]
    }
   ],
   "source": [
    "# Building addition from primitive recursive functions\n",
    "# We have: zero(), successor(), and projection functions\n",
    "\n",
    "# Basic primitive functions\n",
    "def zero():\n",
    "    \"\"\"Z() = 0\"\"\"\n",
    "    return 0\n",
    "\n",
    "def successor(n):\n",
    "    \"\"\"S(n) = n + 1\"\"\"\n",
    "    return n + 1\n",
    "\n",
    "def projection(i, n):\n",
    "    \"\"\"Returns P_i^n - projection function that picks i-th of n arguments\"\"\"\n",
    "    def proj_func(*args):\n",
    "        if len(args) != n:\n",
    "            raise ValueError(f\"Expected {n} arguments, got {len(args)}\")\n",
    "        if i < 1 or i > n:\n",
    "            raise ValueError(f\"Index {i} out of range for {n} arguments\")\n",
    "        return args[i - 1]\n",
    "    return proj_func\n",
    "\n",
    "# Create specific projections we'll need\n",
    "P_1_1 = projection(1, 1)  # Identity function, pick first of one argument\n",
    "P_1_2 = projection(1, 2)  # First of two arguments\n",
    "P_2_2 = projection(2, 2)  # Second of two arguments\n",
    "P_2_3 = projection(2, 3)  # Second of three arguments\n",
    "\n",
    "print(\"=== Step 1: Understanding the recursive definition ===\")\n",
    "print(\"We want to define sum(a, b) using primitive recursion:\")\n",
    "print(\"sum(a, 0) = a\")\n",
    "print(\"sum(a, n+1) = S(sum(a, n))\")\n",
    "print()\n",
    "\n",
    "print(\"=== Step 2: Formal primitive recursive definition ===\")\n",
    "print(\"In primitive recursion, we define a function f by:\")\n",
    "print(\"f(0, x₁, ..., xₖ) = g(x₁, ..., xₖ)         [base case]\")\n",
    "print(\"f(n+1, x₁, ..., xₖ) = h(n, f(n,x₁,...,xₖ), x₁, ..., xₖ)  [recursive case]\")\n",
    "print()\n",
    "print(\"For sum(a, b), we have:\")\n",
    "print(\"- f is our sum function\")\n",
    "print(\"- We're recursing on the second argument b\")\n",
    "print(\"- x₁ = a (the first argument)\")\n",
    "print(\"- So: sum(a, 0) = g(a) and sum(a, n+1) = h(n, sum(a,n), a)\")\n",
    "print()\n",
    "\n",
    "# Step 3: Define the base case function g\n",
    "def g(a):\n",
    "    \"\"\"Base case: sum(a, 0) = a\"\"\"\n",
    "    return P_1_1(a)  # Just return the first (and only) argument\n",
    "\n",
    "print(\"=== Step 3: Base case function g ===\")\n",
    "print(\"g(a) = P_1^1(a) = a\")\n",
    "print(\"This handles: sum(a, 0) = a\")\n",
    "print(f\"Example: g(5) = {g(5)}\")\n",
    "print()\n",
    "\n",
    "# Step 4: Define the recursive case function h\n",
    "def h(n, recursive_result, a):\n",
    "    \"\"\"Recursive case: sum(a, n+1) = S(sum(a, n))\"\"\"\n",
    "    # We want S(recursive_result), which is S(P_2^3(n, recursive_result, a))\n",
    "    return successor(P_2_3(n, recursive_result, a))\n",
    "\n",
    "print(\"=== Step 4: Recursive case function h ===\")\n",
    "print(\"h(n, recursive_result, a) = S(P_2^3(n, recursive_result, a))\")\n",
    "print(\"This handles: sum(a, n+1) = S(sum(a, n))\")\n",
    "print(\"The P_2^3 extracts the recursive_result (sum(a, n))\")\n",
    "print(\"Then S() gives us the successor\")\n",
    "print()\n",
    "\n",
    "# Step 5: Implement the full primitive recursive sum\n",
    "def prim_recursive_sum(a, b):\n",
    "    \"\"\"\n",
    "    Sum function defined by primitive recursion\n",
    "    sum(a, 0) = g(a) = a\n",
    "    sum(a, n+1) = h(n, sum(a,n), a) = S(sum(a,n))\n",
    "    \"\"\"\n",
    "    if b == 0:\n",
    "        return g(a)\n",
    "    else:\n",
    "        # b = n+1 for some n, so n = b-1\n",
    "        n = b - 1\n",
    "        recursive_result = prim_recursive_sum(a, n)\n",
    "        return h(n, recursive_result, a)  # get the successor of `recursive_result\n",
    "\n",
    "print(\"=== Step 5: Testing our primitive recursive sum ===\")\n",
    "test_cases = [(3, 0), (3, 1), (3, 2), (5, 4), (0, 7), (7, 0)]\n",
    "\n",
    "for a, b in test_cases:\n",
    "    result = prim_recursive_sum(a, b)\n",
    "    expected = a + b\n",
    "    print(f\"prim_recursive_sum({a}, {b}) = {result} (expected {expected}) ✓\" if result == expected else \"✗\")\n",
    "\n",
    "print()\n",
    "print(\"=== Step 6: Trace through sum(3, 2) ===\")\n",
    "print(\"sum(3, 2):\")\n",
    "print(\"  Since 2 ≠ 0, we use recursive case with n=1\")\n",
    "print(\"  = h(1, sum(3, 1), 3)\")\n",
    "print(\"  \")\n",
    "print(\"  First we need sum(3, 1):\")\n",
    "print(\"    Since 1 ≠ 0, we use recursive case with n=0\") \n",
    "print(\"    = h(0, sum(3, 0), 3)\")\n",
    "print(\"    \")\n",
    "print(\"    First we need sum(3, 0):\")\n",
    "print(\"      Since 0 = 0, we use base case\")\n",
    "print(\"      = g(3) = P_1^1(3) = 3\")\n",
    "print(\"    \")\n",
    "print(\"    So h(0, 3, 3) = S(P_2^3(0, 3, 3)) = S(3) = 4\")\n",
    "print(\"    Therefore sum(3, 1) = 4\")\n",
    "print(\"  \")\n",
    "print(\"  Now h(1, 4, 3) = S(P_2^3(1, 4, 3)) = S(4) = 5\")\n",
    "print(\"  Therefore sum(3, 2) = 5\")\n",
    "\n",
    "print()\n",
    "print(\"=== Step 7: The key insight ===\")\n",
    "print(\"Addition is primitive recursive because it can be built using only:\")\n",
    "print(\"1. Basic functions: zero(), successor(), projections\")\n",
    "print(\"2. Composition: plugging functions into other functions\")\n",
    "print(\"3. Primitive recursion: the specific pattern above\")\n",
    "print()\n",
    "print(\"No 'loops' or 'general recursion' needed - just this constrained form!\")\n",
    "\n",
    "# Bonus: show that we only used allowed operations\n",
    "print()\n",
    "print(\"=== Verification: Only primitive operations used ===\")\n",
    "print(\"✓ g(a) = P_1^1(a) - uses projection\")\n",
    "print(\"✓ h(n,r,a) = S(P_2^3(n,r,a)) - uses successor and projection\")  \n",
    "print(\"✓ Primitive recursion pattern followed exactly\")\n",
    "print(\"✓ No general recursion, loops, or unbounded search\")"
   ]
  },
  {
   "cell_type": "markdown",
   "id": "0ae01087",
   "metadata": {},
   "source": [
    "## Conditional Logic Using Primitive Recursive Functions\n",
    "It's possible to define conditional logic using primitive recursive functions."
   ]
  },
  {
   "cell_type": "code",
   "execution_count": null,
   "id": "f8b8d78e",
   "metadata": {},
   "outputs": [
    {
     "name": "stdout",
     "output_type": "stream",
     "text": [
      "7 7 7 7\n",
      "9 9 9 9\n"
     ]
    }
   ],
   "source": [
    "# Primitive recursive functions\n",
    "zero, successor = lambda x: 0, lambda x: x + 1\n",
    "\n",
    "# define the boolean functions\n",
    "bool_base = lambda x: zero(x)\n",
    "bool_r = lambda x: successor(zero(x))  # recursive case\n",
    "\n",
    "# Define the complement function.\n",
    "neg_base = lambda x: successor(zero(x))\n",
    "neg_r = lambda x: zero(x)  # recursive case\n",
    "\n",
    "# Pythonic version of the function\n",
    "f = lambda x: 7 if x > 0 else 9\n",
    "\n",
    "# hybrid version\n",
    "f__ = lambda x: 7 * bool(x) + 9 * (bool(not x))\n",
    "\n",
    "# primitive recursive version of the conditional logic\n",
    "f_base = lambda x: 7 * bool_base(x) + 9 * neg_base(bool_base(x))\n",
    "f_rec = lambda x: 7 * bool_r(x) + 9 * neg_r(bool_r(x))\n",
    "\n",
    "\n",
    "def f_explicit(x):\n",
    "    \"\"\"\n",
    "    Define the function f(x) = 7 if x > 0 else 9 step by step to grasp the idea.\n",
    "\n",
    "    Note:\n",
    "    -----\n",
    "    While the logic from the Python version is very straightforward, there's something slippery\n",
    "    here to get this working from first principles, this is to say, the most austere version.\n",
    " \n",
    "    This is kind of circular as we are using conditional logic to define the notion of\n",
    "    conditional logic. But in the recursive world, we would build it from first principles\n",
    "    writing one by one the steps of the recursion.\n",
    "    \"\"\"\n",
    "    if x == 0:  # base case\n",
    "        _bool_base = bool_base(x)  # 0\n",
    "        _neg_base = neg_base(x)  # 1\n",
    "        _bool_base_neg_base = neg_base(_bool_base)  # 1\n",
    "        output = 7 * _bool_base + 9 * _bool_base_neg_base  # 7*0 + 9*1 = 9\n",
    "        return output  # 9\n",
    "    # Recursive case\n",
    "    _bool_r = bool_r(x)  # 1\n",
    "    _neg_r = neg_r(x)  # 0\n",
    "    _bool_r_neg_r = neg_r(_bool_r)  # 0\n",
    "    output = 7 * _bool_r + 9 * _bool_r_neg_r  # 7*1 + 9*0 = 7\n",
    "    return output  # 7\n",
    "\n",
    "print(f(1), f_explicit(1), f_rec(1), f__(1))\n",
    "print(f(0), f_explicit(0), f_base(0), f__(0))\n"
   ]
  },
  {
   "cell_type": "markdown",
   "id": "0ad9ebcd",
   "metadata": {},
   "source": [
    "## For Loops Using Primitive Recursive Functions\n"
   ]
  },
  {
   "cell_type": "code",
   "execution_count": 3,
   "id": "9caa3528",
   "metadata": {},
   "outputs": [
    {
     "data": {
      "text/plain": [
       "'foo'"
      ]
     },
     "execution_count": 3,
     "metadata": {},
     "output_type": "execute_result"
    }
   ],
   "source": [
    "# We have a function R(X) that returns a bool \n",
    "\n",
    "# there's some function r(x)->int:\n",
    "# there's another function R(x)\n",
    "\n",
    "True and 3 or 4\n",
    "\"foo\" * True + \"bar\" * False\n"
   ]
  }
 ],
 "metadata": {
  "kernelspec": {
   "display_name": "lpm-playground",
   "language": "python",
   "name": "python3"
  },
  "language_info": {
   "codemirror_mode": {
    "name": "ipython",
    "version": 3
   },
   "file_extension": ".py",
   "mimetype": "text/x-python",
   "name": "python",
   "nbconvert_exporter": "python",
   "pygments_lexer": "ipython3",
   "version": "3.13.0"
  }
 },
 "nbformat": 4,
 "nbformat_minor": 5
}
